quarantine 3/n: SlabsCommon.fsti

src/SlabsCommon.fsti
@@ -51,6 +51,7 @@ let pred1 (x: U32.t) : prop = U32.eq x 0ul == true
 let pred2 (x: U32.t) : prop = U32.eq x 1ul == true
 let pred3 (x: U32.t) : prop = U32.eq x 2ul == true
 let pred4 (x: U32.t) : prop = U32.eq x 3ul == true
+let pred5 (x: U32.t) : prop = U32.eq x 4ul == true
 
 /// If the sequence is partitioned into three lists, then any
 /// element satisfying pred2 belongs to the second list.
@@ -58,27 +59,30 @@ let pred4 (x: U32.t) : prop = U32.eq x 3ul == true
 /// are mutually exclusive, which is why we include this lemma
 /// here instead of in the ArrayListGen library.
 let lemma_partition_and_pred_implies_mem2
-  (hd1 hd2 hd3 hd4:nat)
+  (hd1 hd2 hd3 hd4 hd5:nat)
   (s:Seq.seq AL.cell)
   (idx:nat{idx < Seq.length s})
   : Lemma
     (requires
       idx <> ALG.null /\
-      ALG.partition s hd1 hd2 hd3 hd4 /\
-      ALG.varraylist_refine pred1 pred2 pred3 pred4 hd1 hd2 hd3 hd4 s /\
+      ALG.partition s hd1 hd2 hd3 hd4 hd5 /\
+      ALG.varraylist_refine pred1 pred2 pred3 pred4 pred5
+        hd1 hd2 hd3 hd4 hd5 s /\
       pred2 (ALG.get_data (Seq.index s idx)))
     (ensures ALG.mem idx hd2 s)
   = ALG.lemma_mem_ptrs_in hd1 s idx;
     ALG.lemma_mem_ptrs_in hd2 s idx;
     ALG.lemma_mem_ptrs_in hd3 s idx;
     ALG.lemma_mem_ptrs_in hd4 s idx;
+    ALG.lemma_mem_ptrs_in hd5 s idx;
     let open FStar.FiniteSet.Ambient in
     (* Need this assert to trigger the right SMTPats in FiniteSet.Ambiant *)
-    assert (FStar.FiniteSet.Base.mem idx (ALG.ptrs_all hd1 hd2 hd3 hd4 s));
+    assert (FStar.FiniteSet.Base.mem idx (ALG.ptrs_all hd1 hd2 hd3 hd4 hd5 s));
     Classical.move_requires (ALG.lemma_mem_implies_pred pred1 hd1 s) idx;
     Classical.move_requires (ALG.lemma_mem_implies_pred pred2 hd2 s) idx;
     Classical.move_requires (ALG.lemma_mem_implies_pred pred3 hd3 s) idx;
-    Classical.move_requires (ALG.lemma_mem_implies_pred pred4 hd4 s) idx
+    Classical.move_requires (ALG.lemma_mem_implies_pred pred4 hd4 s) idx;
+    Classical.move_requires (ALG.lemma_mem_implies_pred pred5 hd5 s) idx
 
 /// If the sequence is partitioned into three lists, then any
 /// element satisfying pred3 belongs to the third list.
@@ -86,27 +90,30 @@ let lemma_partition_and_pred_implies_mem2
 /// are mutually exclusive, which is why we include this lemma
 /// here instead of in the ArrayListGen library.
 let lemma_partition_and_pred_implies_mem3
-  (hd1 hd2 hd3 hd4:nat)
+  (hd1 hd2 hd3 hd4 hd5:nat)
   (s:Seq.seq AL.cell)
   (idx:nat{idx < Seq.length s})
   : Lemma
     (requires
       idx <> ALG.null /\
-      ALG.partition s hd1 hd2 hd3 hd4 /\
-      ALG.varraylist_refine pred1 pred2 pred3 pred4 hd1 hd2 hd3 hd4 s /\
+      ALG.partition s hd1 hd2 hd3 hd4 hd5 /\
+      ALG.varraylist_refine pred1 pred2 pred3 pred4 pred5
+        hd1 hd2 hd3 hd4 hd5 s /\
       pred3 (ALG.get_data (Seq.index s idx)))
     (ensures ALG.mem idx hd3 s)
   = ALG.lemma_mem_ptrs_in hd1 s idx;
     ALG.lemma_mem_ptrs_in hd2 s idx;
     ALG.lemma_mem_ptrs_in hd3 s idx;
     ALG.lemma_mem_ptrs_in hd4 s idx;
+    ALG.lemma_mem_ptrs_in hd5 s idx;
     let open FStar.FiniteSet.Ambient in
     (* Need this assert to trigger the right SMTPats in FiniteSet.Ambiant *)
-    assert (FStar.FiniteSet.Base.mem idx (ALG.ptrs_all hd1 hd2 hd3 hd4 s));
+    assert (FStar.FiniteSet.Base.mem idx (ALG.ptrs_all hd1 hd2 hd3 hd4 hd5 s));
     Classical.move_requires (ALG.lemma_mem_implies_pred pred1 hd1 s) idx;
     Classical.move_requires (ALG.lemma_mem_implies_pred pred2 hd2 s) idx;
     Classical.move_requires (ALG.lemma_mem_implies_pred pred3 hd3 s) idx;
-    Classical.move_requires (ALG.lemma_mem_implies_pred pred4 hd4 s) idx
+    Classical.move_requires (ALG.lemma_mem_implies_pred pred4 hd4 s) idx;
+    Classical.move_requires (ALG.lemma_mem_implies_pred pred5 hd5 s) idx
 
 open Guards
 
@@ -143,6 +150,13 @@ let p_guard (size_class) : blob -> vprop
     slab_vprop size_class (snd b) (fst b)
     `VR2.vrefine`
     (is_guard size_class (snd b) (fst b))
+
+let p_quarantine (size_class) : blob -> vprop
+  =
+  fun (b:blob) ->
+    slab_vprop size_class (snd b) (fst b)
+    `VR2.vrefine`
+    (is_quarantine size_class (snd b) (fst b))
 
 val p_empty_unpack (#opened:_)
   (sc: sc)
@@ -217,6 +231,24 @@ val p_guard_unpack (#opened:_)
     b1 == b2 /\
     is_guard sc (snd b1) (fst b1) blob1 /\
     h0 ((p_guard sc) b1)
+    ==
+    h1 (slab_vprop sc (snd b2) (fst b2))
+  )
+
+val p_quarantine_unpack (#opened:_)
+  (sc: sc)
+  (b1 b2: blob)
+  : SteelGhost unit opened
+  ((p_quarantine sc) b1)
+  (fun _ -> slab_vprop sc (snd b2) (fst b2))
+  (requires fun _ -> b1 == b2)
+  (ensures fun h0 _ h1 ->
+    let blob1
+      : t_of (slab_vprop sc (snd b2) (fst b2))
+      = h1 (slab_vprop sc (snd b2) (fst b2)) in
+    b1 == b2 /\
+    is_quarantine sc (snd b1) (fst b1) blob1 /\
+    h0 ((p_quarantine sc) b1)
     ==
     h1 (slab_vprop sc (snd b2) (fst b2))
   )
@@ -304,6 +336,27 @@ val p_guard_pack (#opened:_)
   (ensures fun h0 _ h1 ->
     b1 == b2 /\
     h1 ((p_guard sc) b2)
+    ==
+    h0 (slab_vprop sc (snd b1) (fst b1))
+  )
+
+val p_quarantine_pack (#opened:_)
+  (sc: sc)
+  (b1: blob)
+  (b2: blob)
+  : SteelGhost unit opened
+  (slab_vprop sc (snd b1) (fst b1))
+  (fun _ -> (p_quarantine sc) b2)
+  (requires fun h0 ->
+    let blob0
+      : t_of (slab_vprop sc (snd b1) (fst b1))
+      = h0 (slab_vprop sc (snd b1) (fst b1)) in
+    is_quarantine sc (snd b1) (fst b1) blob0 /\
+    b1 == b2
+  )
+  (ensures fun h0 _ h1 ->
+    b1 == b2 /\
+    h1 ((p_quarantine sc) b2)
     ==
     h0 (slab_vprop sc (snd b1) (fst b1))
   )
@@ -417,6 +470,7 @@ let f
   | 1ul -> p_partial size_class (md_bm_array md_bm_region i, slab_array slab_region i)
   | 2ul -> p_full size_class (md_bm_array md_bm_region i, slab_array slab_region i)
   | 3ul -> p_guard size_class (md_bm_array md_bm_region i, slab_array slab_region i)
+  | 4ul -> p_quarantine size_class (md_bm_array md_bm_region i, slab_array slab_region i)
 
 val t (size_class: sc) : Type0
 
@@ -432,50 +486,57 @@ val f_lemma
   == t size_class)
 
 let ind_varraylist_aux2
-  (pred1 pred2 pred3 pred4: AL.status -> prop) (r: A.array AL.cell)
-  (idxs: ((US.t & US.t) & US.t) & US.t)
+  (r: A.array AL.cell)
+  (idxs: (((US.t & US.t) & US.t) & US.t) & US.t)
   =
-  AL.varraylist pred1 pred2 pred3 pred4 r
-    (US.v (fst (fst (fst idxs))))
+  AL.varraylist pred1 pred2 pred3 pred4 pred5 r
+    (US.v (fst (fst (fst (fst idxs)))))
+    (US.v (snd (fst (fst (fst idxs)))))
     (US.v (snd (fst (fst idxs))))
     (US.v (snd (fst idxs)))
     (US.v (snd idxs))
 
 let ind_varraylist_aux_refinement
-  (pred1 pred2 pred3 pred4: AL.status -> prop) (r: A.array AL.cell)
-  (idxs: ((US.t & US.t) & US.t) & US.t)
-  (s: t_of (ind_varraylist_aux2 pred1 pred2 pred3 pred4 r idxs))
+  (r: A.array AL.cell)
+  (idxs: (((US.t & US.t) & US.t) & US.t) & US.t)
+  (s: t_of (ind_varraylist_aux2 r idxs))
   : prop
   =
   ALG.partition #AL.status s
-    (US.v (fst (fst (fst idxs))))
+    (US.v (fst (fst (fst (fst idxs)))))
+    (US.v (snd (fst (fst (fst idxs)))))
     (US.v (snd (fst (fst idxs))))
     (US.v (snd (fst idxs)))
     (US.v (snd idxs))
 
 let ind_varraylist_aux
-  (pred1 pred2 pred3 pred4: AL.status -> prop) (r: A.array AL.cell)
-  (idxs: ((US.t & US.t) & US.t) & US.t)
+  (r: A.array AL.cell)
+  (idxs: (((US.t & US.t) & US.t) & US.t) & US.t)
   =
-  ind_varraylist_aux2 pred1 pred2 pred3 pred4 r idxs
+  ind_varraylist_aux2 r idxs
   `vrefine`
-  ind_varraylist_aux_refinement pred1 pred2 pred3 pred4 r idxs
+  ind_varraylist_aux_refinement r idxs
 
 let ind_varraylist
-  (pred1 pred2 pred3 pred4: AL.status -> prop) (r: A.array AL.cell)
-  (r1 r2 r3 r4: ref US.t)
+  (r: A.array AL.cell)
+  (r1 r2 r3 r4 r5: ref US.t)
   =
-  (vptr r1 `star` vptr r2 `star` vptr r3 `star` vptr r4) `vdep`
-  ind_varraylist_aux pred1 pred2 pred3 pred4 r
+  (
+    vptr r1 `star`
+    vptr r2 `star`
+    vptr r3 `star`
+    vptr r4 `star`
+    vptr r5
+  ) `vdep` ind_varraylist_aux r
 
 let left_vprop1
   (md_region: array AL.cell{A.length md_region = US.v metadata_max})
-  (r1 r2 r3 r4: ref US.t)
+  (r1 r2 r3 r4 r5: ref US.t)
   (md_count_v: US.t{US.v md_count_v <= US.v metadata_max})
   =
-  ind_varraylist pred1 pred2 pred3 pred4
+  ind_varraylist
     (A.split_l md_region md_count_v)
-    r1 r2 r3 r4
+    r1 r2 r3 r4 r5
 
 let left_vprop2
   (size_class: sc)
@@ -496,9 +557,9 @@ let left_vprop_aux
   (slab_region: array U8.t{A.length slab_region = US.v metadata_max * U32.v page_size})
   (md_bm_region: array U64.t{A.length md_bm_region = US.v metadata_max * 4})
   (md_region: array AL.cell{A.length md_region = US.v metadata_max})
-  (r1 r2 r3 r4: ref US.t)
+  (r1 r2 r3 r4 r5: ref US.t)
   (md_count_v: US.t{US.v md_count_v <= US.v metadata_max})
-  (x: t_of (ind_varraylist pred1 pred2 pred3 pred4 (A.split_l md_region md_count_v) r1 r2 r3 r4))
+  (x: t_of (ind_varraylist (A.split_l md_region md_count_v) r1 r2 r3 r4 r5))
   = starseq
       #(pos:US.t{US.v pos < US.v md_count_v})
       #(t size_class)
@@ -511,12 +572,12 @@ let left_vprop
   (slab_region: array U8.t{A.length slab_region = US.v metadata_max * U32.v page_size})
   (md_bm_region: array U64.t{A.length md_bm_region = US.v metadata_max * 4})
   (md_region: array AL.cell{A.length md_region = US.v metadata_max})
-  (r1 r2 r3 r4: ref US.t)
+  (r1 r2 r3 r4 r5: ref US.t)
   (md_count_v: US.t{US.v md_count_v <= US.v metadata_max})
   =
-  left_vprop1 md_region r1 r2 r3 r4 md_count_v
+  left_vprop1 md_region r1 r2 r3 r4 r5 md_count_v
   `vdep`
-  left_vprop_aux size_class slab_region md_bm_region md_region r1 r2 r3 r4 md_count_v
+  left_vprop_aux size_class slab_region md_bm_region md_region r1 r2 r3 r4 r5 md_count_v
 
 unfold
 let vrefinedep_prop (x:US.t) : prop =
@@ -541,13 +602,13 @@ let size_class_vprop_aux
   (slab_region: array U8.t{A.length slab_region = US.v metadata_max * U32.v page_size})
   (md_bm_region: array U64.t{A.length md_bm_region = US.v metadata_max * 4})
   (md_region: array AL.cell{A.length md_region = US.v metadata_max})
-  empty_slabs partial_slabs full_slabs guard_slabs
+  empty_slabs partial_slabs full_slabs guard_slabs quarantine_slabs
   (v: US.t{US.v v <= US.v metadata_max == true})
   : vprop
   =
   left_vprop size_class
     slab_region md_bm_region md_region
-    empty_slabs partial_slabs full_slabs guard_slabs v `star`
+    empty_slabs partial_slabs full_slabs guard_slabs quarantine_slabs v `star`
   right_vprop
     slab_region md_bm_region md_region v
 
@@ -560,10 +621,10 @@ val pack_3
   (md_bm_region: array U64.t{A.length md_bm_region = US.v metadata_max * 4})
   (md_region: array AL.cell{A.length md_region = US.v metadata_max})
   (md_count: ref US.t)
-  (r1 r2 r3 r4: ref US.t)
+  (r1 r2 r3 r4 r5: ref US.t)
   (md_count_v: US.t{US.v md_count_v <= US.v metadata_max})
   (md_region_lv: G.erased (Seq.lseq AL.status (US.v md_count_v)))
-  (idx1 idx2 idx3 idx4: US.t)
+  (idx1 idx2 idx3 idx4 idx5: US.t)
   : SteelGhost unit opened
   (
     vptr md_count `star`
@@ -571,9 +632,10 @@ val pack_3
     vptr r2 `star`
     vptr r3 `star`
     vptr r4 `star`
-    (AL.varraylist pred1 pred2 pred3 pred4
+    vptr r5 `star`
+    (AL.varraylist pred1 pred2 pred3 pred4 pred5
       (A.split_l md_region md_count_v)
-      (US.v idx1) (US.v idx2) (US.v idx3) (US.v idx4)) `star`
+      (US.v idx1) (US.v idx2) (US.v idx3) (US.v idx4) (US.v idx5)) `star`
     starseq
       #(pos:US.t{US.v pos < US.v md_count_v})
       #(t size_class)
@@ -585,28 +647,29 @@ val pack_3
     vrefinedep
       (vptr md_count)
       vrefinedep_prop
-      (left_vprop size_class slab_region md_bm_region md_region r1 r2 r3 r4)
+      (left_vprop size_class slab_region md_bm_region md_region r1 r2 r3 r4 r5)
   )
   (requires fun h0 ->
-    let gs0 = AL.v_arraylist pred1 pred2 pred3 pred4
+    let gs0 = AL.v_arraylist pred1 pred2 pred3 pred4 pred5
       (A.split_l md_region md_count_v)
-      (US.v idx1) (US.v idx2) (US.v idx3) (US.v idx4) h0 in
+      (US.v idx1) (US.v idx2) (US.v idx3) (US.v idx4) (US.v idx5) h0 in
     US.v md_count_v <> AL.null /\
     sel md_count h0 == md_count_v /\
     sel r1 h0 == idx1 /\
     sel r2 h0 == idx2 /\
     sel r3 h0 == idx3 /\
     sel r4 h0 == idx4 /\
+    sel r5 h0 == idx5 /\
     ALG.dataify gs0 `Seq.equal` G.reveal md_region_lv /\
     ALG.partition #AL.status gs0
-      (US.v idx1) (US.v idx2) (US.v idx3) (US.v idx4)
+      (US.v idx1) (US.v idx2) (US.v idx3) (US.v idx4) (US.v idx5)
   )
   (ensures fun _ _ h1 ->
     let blob1
       = h1 (vrefinedep
       (vptr md_count)
       vrefinedep_prop
-      (left_vprop size_class slab_region md_bm_region md_region r1 r2 r3 r4)
+      (left_vprop size_class slab_region md_bm_region md_region r1 r2 r3 r4 r5)
     ) in
     md_count_v == dfst blob1)
 
@@ -617,7 +680,7 @@ val pack_slab_starseq
   (md_bm_region: array U64.t{A.length md_bm_region = US.v metadata_max * 4})
   (md_region: array AL.cell{A.length md_region = US.v metadata_max})
   (md_count: ref US.t)
-  (r1 r2 r3 r4: ref US.t)
+  //(r1 r2 r3 r4 r5: ref US.t)
   (md_count_v: US.t{US.v md_count_v <= US.v metadata_max})
   (md_region_lv: G.erased (Seq.lseq AL.status (US.v md_count_v)))
   (idx: US.t{US.v idx < US.v md_count_v})
@@ -657,6 +720,9 @@ val pack_slab_starseq
       (md_bm_array md_bm_region idx)) in
     let md : Seq.lseq U64.t 4 = dfst md_blob in
     //(v == 3ul ==> is_guard size_class md) /\
+    (v == 4ul ==> is_quarantine  size_class
+      (slab_array slab_region idx)
+      (md_bm_array md_bm_region idx) md_blob) /\
     (v == 3ul ==> is_guard size_class
       (slab_array slab_region idx)
       (md_bm_array md_bm_region idx) md_blob) /\
@@ -674,14 +740,14 @@ val pack_right_and_refactor_vrefine_dep
   (md_bm_region: array U64.t{A.length md_bm_region = US.v metadata_max * 4})
   (md_region: array AL.cell{A.length md_region = US.v metadata_max})
   (md_count: ref US.t)
-  (r1 r2 r3 r4: ref US.t)
+  (r1 r2 r3 r4 r5: ref US.t)
   (md_count_v: US.t{US.v md_count_v <= US.v metadata_max})
   : SteelGhost unit opened
   (
     vrefinedep
       (vptr md_count)
       vrefinedep_prop
-      (left_vprop size_class slab_region md_bm_region md_region r1 r2 r3 r4)
+      (left_vprop size_class slab_region md_bm_region md_region r1 r2 r3 r4 r5)
     `star`
     right_vprop slab_region md_bm_region md_region md_count_v
   )
@@ -689,14 +755,14 @@ val pack_right_and_refactor_vrefine_dep
     vrefinedep
       (vptr md_count)
       vrefinedep_prop
-      (size_class_vprop_aux size_class slab_region md_bm_region md_region r1 r2 r3 r4)
+      (size_class_vprop_aux size_class slab_region md_bm_region md_region r1 r2 r3 r4 r5)
   )
   (requires fun h0 ->
     let blob0
       = h0 (vrefinedep
       (vptr md_count)
       vrefinedep_prop
-      (left_vprop size_class slab_region md_bm_region md_region r1 r2 r3 r4)
+      (left_vprop size_class slab_region md_bm_region md_region r1 r2 r3 r4 r5)
     ) in
     md_count_v == dfst blob0)
   (ensures fun h0 _ h1 ->
@@ -704,13 +770,13 @@ val pack_right_and_refactor_vrefine_dep
       = h0 (vrefinedep
       (vptr md_count)
       vrefinedep_prop
-      (left_vprop size_class slab_region md_bm_region md_region r1 r2 r3 r4)
+      (left_vprop size_class slab_region md_bm_region md_region r1 r2 r3 r4 r5)
     ) in
     let blob1
       = h1 (vrefinedep
       (vptr md_count)
       vrefinedep_prop
-      (size_class_vprop_aux size_class slab_region md_bm_region md_region r1 r2 r3 r4)
+      (size_class_vprop_aux size_class slab_region md_bm_region md_region r1 r2 r3 r4 r5)
     ) in
     dfst blob0 == dfst blob1
   )
